formal/CclFormal.lean
@@ -3,3 +3,5 @@ import CclFormal.Sub
 import CclFormal.Decide
 import CclFormal.Json
 import CclFormal.Props
+import CclFormal.Equiv
+import CclFormal.Trans
